Coq: add some properties to the bitvector interface

lib/coq/MachineWordBBV.v
@@ -17,14 +17,120 @@ Qed.
 Definition cast_word {m n} (x : Word.word m) (eq : m = n) : Word.word n :=
   DepEqNat.nat_cast _ eq x.
 
+Lemma cast_word_refl n (w : Word.word n) :
+  cast_word w eq_refl = w.
+apply DepEqNat.nat_cast_same.
+Qed.
+
 Definition word := Word.word.
 Definition zeros n : word n := @Word.wzero n.
 Definition ones n : word n := @Word.wones n.
-Definition get_bit [n] : word n -> nat -> bool :=
+Fixpoint get_bit [n] (w : word n) : nat -> bool :=
+  match w with
+  | Word.WO => fun i => dummy false
+  | Word.WS b w' => fun i =>
+             match i with
+             | O => b
+             | S i' => get_bit w' i'
+             end
+  end.
+
+Lemma get_bit_eq [n] (w v : word n) :
+  (forall i, i < n -> get_bit w i = get_bit v i) -> w = v.
+intro H.
+induction w.
+* rewrite (Word.word0 v).
+  reflexivity.
+* unfold word in v.
+  rewrite (Word.shatter_word v) in *.
+  f_equal.
+  + apply (H 0).
+    Lia.lia.
+  + apply IHw.
+    intros i LT.
+    specialize (H (S i) ltac:(Lia.lia)).
+    apply H.
+Qed.
+
+(* An alternative definition in the style of set_bit below. *)
+Definition get_bit_by_shift [n] : word n -> nat -> bool :=
   match n with
   | O => fun (w : Word.word O) i => dummy false
   | S n => fun (w : Word.word (S n)) i => Word.wlsb (Word.wrshift' w i)
   end.
+
+Lemma combine_bit_low : forall m n (w : word m) (v : word n) i,
+  i < m -> get_bit (Word.combine w v) i = get_bit w i.
+induction w.
+* intros.
+  Lia.lia.
+* intros v [|i] LT.
+  + reflexivity.
+  + apply IHw.
+    Lia.lia.
+Qed.
+
+Lemma combine_bit_high : forall m n (w : word m) (v : word n) i,
+  get_bit (Word.combine w v) (i + m) = get_bit v i.
+induction w.
+* intros.
+  simpl.
+  rewrite Nat.add_0_r.
+  reflexivity.
+* intros.
+  rewrite Nat.add_succ_r.
+  apply IHw.
+Qed.
+
+Lemma split2_bit : forall m n w i,
+get_bit (Word.split2 m n w) i = get_bit w (i + m).
+induction m.
+* intros.
+  rewrite Nat.add_0_r.
+  reflexivity.
+* simpl. intros.
+  rewrite (Word.shatter_word w) at 2.
+  rewrite Nat.add_succ_r.
+  apply IHm.
+Qed.
+
+Lemma nat_cast_bit : forall m n (w : word m) (H : m = n) i,
+  get_bit (DepEqNat.nat_cast Word.word H w) i = get_bit w i.
+intros.
+subst.
+rewrite DepEqNat.nat_cast_same.
+reflexivity.
+Qed.
+
+Lemma wrshift_bit : forall n (w : word n) i j,
+  i + j < n ->
+  get_bit (Word.wrshift' w i) j = get_bit w (i + j).
+intros.
+unfold Word.wrshift'.
+rewrite split2_bit.
+rewrite nat_cast_bit.
+rewrite (Nat.add_comm j i).
+apply combine_bit_low.
+assumption.
+Qed.
+
+Lemma wlsb_bit : forall n (w : word (S n)),
+  Word.wlsb w = get_bit w 0.
+intros.
+rewrite (Word.shatter_word w).
+reflexivity.
+Qed.
+
+Lemma get_bit_equiv : forall n (w : word n) i, i < n -> get_bit w i = get_bit_by_shift w i.
+destruct w.
+* intros.
+  reflexivity.
+* intros.
+  simpl (get_bit_by_shift _ _).
+  rewrite wlsb_bit.
+  rewrite wrshift_bit; auto.
+  Lia.lia.
+Qed.
 
 Definition set_bit [n] : word n -> nat -> bool -> word n :=
 match n with
@@ -64,6 +170,89 @@ end.
 
 Definition word_to_bools [n] (w : word n) : list bool := word_to_bools_aux w [].
 
+Local Lemma word_to_bools_aux_nth : forall n (w : word n) l i,
+  List.nth_error (word_to_bools_aux w l) (n + i) = List.nth_error l i.
+induction w.
+* reflexivity.
+* intros.
+  simpl (word_to_bools_aux _ _).
+  rewrite Nat.add_succ_comm.
+  rewrite IHw.
+  reflexivity.
+Qed.
+
+Lemma word_to_bools_length : forall [n] (w : word n), List.length (word_to_bools w) = n.
+intros.
+unfold word_to_bools.
+rewrite plus_n_O.
+change 0 with (List.length ([] : list bool)).
+generalize (@nil bool).
+induction n.
+* dependent inversion w.
+  reflexivity.
+* intro.
+  dependent inversion w; subst.
+  simpl.
+  rewrite IHn.
+  simpl.
+  apply Nat.add_succ_r.
+Qed.
+
+Lemma word_to_bools_get_bit : forall [n] (w : word n) (i : nat) x,
+  List.nth_error (word_to_bools w) i = Some x <-> get_bit w (n - i - 1) = x /\ i < n.
+intros.
+split.
+- intro H.
+  specialize (List.nth_error_Some (word_to_bools w) i) as [LEN _].
+  rewrite H in LEN.
+  specialize (LEN ltac:(congruence)).
+  rewrite word_to_bools_length in LEN.
+  split; [|assumption].
+
+  unfold word_to_bools in H.
+  revert H.
+  generalize (@nil bool).
+  induction w.
+  * Lia.lia.
+  * destruct (Nat.eq_dec i n).
+    + subst.
+      intros.
+      assert (x = b). {
+        clear -H.
+        revert H.
+        simpl.
+        rewrite (plus_n_O n) at 2.
+        rewrite word_to_bools_aux_nth.
+        simpl. congruence.
+      }
+      subst.
+      replace (S n - n - 1) with 0 by Lia.lia.
+      reflexivity.
+    + replace (S n - i - 1) with (S (n - i - 1)) by Lia.lia.
+      simpl.
+      intros.
+      apply IHw with (l := List.cons b l); [Lia.lia|].
+      assumption.
+- intros [GET LT].
+  unfold word_to_bools.
+  generalize (@nil bool).
+  induction w.
+  * Lia.lia.
+  * destruct (Nat.eq_dec i n).
+    + subst.
+      intro.
+      rewrite (plus_n_O n) at 3.
+      simpl (word_to_bools_aux _ _).
+      rewrite word_to_bools_aux_nth.
+      replace (S n - n - 1) with 0 by Lia.lia.
+      reflexivity.
+    + intro.
+      simpl (word_to_bools_aux _ _).
+      apply IHw; [|Lia.lia].
+      replace (S n - i - 1) with (S (n - i - 1)) in GET by Lia.lia.
+      apply GET.
+Qed.
+
 Fixpoint bools_to_word_rev l : word (length l) :=
 match l with
 | [] => Word.WO
@@ -71,6 +260,140 @@ match l with
 end%list.
 Definition bools_to_word l : word (length l) :=
   cast_word (bools_to_word_rev (List.rev l)) (List.rev_length l).
+
+Lemma get_bit_cast_word m n (w : word m) (E : m = n) i :
+  get_bit (cast_word w E) i = get_bit w i.
+subst.
+rewrite cast_word_refl.
+reflexivity.
+Qed.
+
+Local Lemma bools_to_word_rev_get_bit : forall l i b,
+  List.nth_error l i = Some b <-> get_bit (bools_to_word_rev l) i = b /\ i < length l.
+induction l.
+* destruct i; intros; split; simpl; intro; solve [congruence|Lia.lia].
+* intros.
+  destruct i.
+  - simpl. intuition; solve [ congruence | Lia.lia ].
+  - simpl. rewrite IHl.
+    intuition.
+Qed.
+
+Lemma nth_error_rev A (l : list A) i x :
+  List.nth_error l i = Some x <-> List.nth_error (List.rev l) (length l - i - 1) = Some x /\ i < length l.
+destruct (lt_dec i (length l)) as [H|H].
+* rewrite List.nth_error_nth' with (d := x); auto.
+  rewrite List.nth_error_nth' with (d := x). 2: {
+    rewrite List.rev_length.
+    Lia.lia.
+  }
+  rewrite List.rev_nth. 2: Lia.lia.
+  replace (length l - S (length l - i - 1)) with i by Lia.lia.
+  tauto.
+* apply not_lt in H.
+  specialize (List.nth_error_None l i) as H'.
+  intuition; solve [congruence | Lia.lia].
+Qed.
+
+Lemma bools_to_word_get_bit : forall l i b,
+  List.nth_error l i = Some b <-> get_bit (bools_to_word l) (length l - i - 1) = b /\ i < length l.
+intros.
+unfold bools_to_word.
+rewrite get_bit_cast_word.
+rewrite nth_error_rev.
+rewrite bools_to_word_rev_get_bit.
+intuition.
+rewrite List.rev_length.
+Lia.lia.
+Qed.
+
+Lemma wrshift_alt : forall sz (w: word sz) n, Word.wrshift' w n = Word.wrshift w n.
+intros.
+unfold Word.wrshift, Word.wrshift'.
+f_equal.
+generalize (Word.combine w (Word.wzero n)).
+generalize (Nat.add_comm sz n).
+generalize (Nat.add_comm n sz).
+generalize (sz + n).
+intros n' e.
+subst.
+intros.
+rewrite DepEqNat.nat_cast_proof_irrel with (e2 := eq_refl).
+rewrite DepEqNat.nat_cast_same.
+reflexivity.
+Qed.
+
+Lemma wzero_msb : forall sz H, Word.wzero (S sz) = eq_rect _ _ (Word.combine (Word.wzero sz) (Word.wzero 1)) _ H.
+induction sz.
+* simpl. intros [].
+  reflexivity.
+* intros H.
+  change (Word.wzero (S (S sz))) with (Word.WS false (Word.wzero (S sz))).
+  erewrite IHsz at 1.
+  erewrite <- Word.WS_eq_rect.
+  eapply eq_refl.
+  Unshelve.
+  Lia.lia.
+Qed.
+
+Lemma word_to_N_get_bit : forall [n] (w: word n) i, i < n -> get_bit w i = N.testbit (word_to_N w) (N.of_nat i).
+unfold word_to_N.
+intros n w i; revert n w.
+induction i.
+* intros.
+  dependent inversion w as [|b n' w']; subst.
+  + Lia.lia.
+  + simpl.
+    destruct b; destruct (Word.wordToN w'); reflexivity.
+* intros n w LT.
+  dependent inversion w as [|b n' w']; subst.
+  + Lia.lia.
+  + simpl (get_bit _ _).
+    simpl (Word.wordToN _).
+    rewrite IHi; [|Lia.lia].
+    rewrite Nat2N.inj_succ.
+    destruct b.
+    - destruct (Word.wordToN w');
+      rewrite N.testbit_succ_r_div2; auto; Lia.lia.
+    - destruct (Word.wordToN w');
+      rewrite N.testbit_succ_r_div2; auto; Lia.lia.
+Qed.
+
+Lemma testbit_word_to_N_high : forall [n] (w: word n) i, (i >= N.of_nat n)%N ->
+  N.testbit (word_to_N w) i = false.
+induction w.
+* reflexivity.
+* intros i I.
+  replace (word_to_N (Word.WS b w)) with (2 * (word_to_N w) + N.b2n b)%N. 2: {
+    destruct b; simpl; destruct (word_to_N w); reflexivity.
+  }
+  destruct (N.zero_or_succ i) as [|[j J]]. Lia.lia.
+  subst.
+  rewrite N.testbit_succ_r.
+  apply IHw.
+  Lia.lia.
+Qed.
+ 
+Lemma word_to_bools_nth_Some : forall [n] (w : word n) (i : nat) x, n > 0 ->
+  List.nth_error (word_to_bools w) i = Some x <-> x = N.testbit (word_to_N w) (N.of_nat (n - i - 1)) /\ i < n.
+intros.
+rewrite word_to_bools_get_bit.
+rewrite word_to_N_get_bit.
+intuition.
+Lia.lia.
+Qed.
+
+Lemma bools_to_word_nth_Some : forall (l : list bool) i b,
+  List.nth_error l i = Some b <-> b = N.testbit (word_to_N (bools_to_word l)) (N.of_nat (length l - i - 1)) /\ i < length l.
+intros.
+destruct l.
+* destruct i; simpl; intuition; congruence.
+* rewrite bools_to_word_get_bit.
+  rewrite word_to_N_get_bit.
+  intuition.
+  simpl (length _).
+  Lia.lia.
+Qed.
 
 Local Lemma slice_equality {i n m} : i + n <= m -> m = i + (n + (m - n -i)).
 Lia.lia.
