lib/coq/MachineWordStdpp.v
@@ -11,6 +11,20 @@ Definition zeros n : word n := bitvector.bv_0 (N.of_nat n).
 
 Definition get_bit [n] (w : word n) i : bool := Z.testbit (bitvector.bv_unsigned w) (Z.of_nat i).
 
+Lemma get_bit_eq : forall [n] (w v : word n),
+  (forall i, i < n -> get_bit w i = get_bit v i) -> w = v.
+intros n w v H.
+apply bitvector.bv_eq.
+unfold get_bit in *.
+apply Z.bits_inj'.
+intros m LE.
+destruct (Z_lt_dec m (Z.of_nat n)).
+* rewrite <- (Z2Nat.id m LE).
+  apply H.
+  Lia.lia.
+* rewrite !bitvector.bv_unsigned_spec_high; auto; Lia.lia.
+Qed.
+
 Definition word_to_Z [n] (w : word n) : Z := bitvector.bv_signed w.
 Definition word_to_N [n] (w : word n) : N := Z.to_N (bitvector.bv_unsigned w).
 Definition Z_to_word n z : word n := bitvector.Z_to_bv _ z.
@@ -25,6 +39,22 @@ intros [LE LT].
 unfold word_to_N.
 rewrite <- (N2Z.id (2 ^ N.of_nat n)).
 rewrite <- Z2N.inj_lt;  Lia.lia.
+Qed.
+
+(* TODO: this proof is generic, should be shared *)
+Lemma testbit_word_to_N_high : forall [n] (w: word n) i, (i >= N.of_nat n)%N ->
+  N.testbit (word_to_N w) i = false.
+intros.
+specialize (word_to_N_range w).
+generalize (word_to_N w) as m.
+intros.
+destruct (N.testbit_spec m i) as [l [h [H1 H2]]].
+destruct (N.testbit m i).
+* simpl (N.b2n true) in H2. subst.
+  assert (l + (1 + 2 * h) * 2 ^ i >= 2 ^ i)%N by Lia.lia.
+  specialize (N.pow_le_mono_r 2 (N.of_nat n) i).
+  Lia.lia.
+* reflexivity.
 Qed.
 
 Lemma word_to_Z_range : forall [n] (w : word (S n)), (- 2 ^ Z.of_nat n <= word_to_Z w < 2 ^ Z.of_nat n)%Z.
@@ -46,6 +76,135 @@ Definition ones n : word n := bitvector.Z_to_bv _ (-1).
 
 Definition word_to_bools [n] (w : word n) : list bool := List.rev (bitvector.bv_to_bits w).
 Definition bools_to_word (l : list bool) : word (List.length l) := N_to_word (List.length l) (Ascii.N_of_digits (List.rev l)).
+
+Lemma word_to_bools_length : forall [n] (w : word n), List.length (word_to_bools w) = n.
+intros.
+unfold word_to_bools.
+rewrite List.rev_length.
+rewrite bitvector.bv_to_bits_length.
+apply Nnat.Nat2N.id.
+Qed.
+
+Lemma nth_error_lookup {A} (l : list A) (i : nat) :
+  base.lookup i l = List.nth_error l i.
+destruct (List.nth_error l i) eqn:H.
+* specialize (List.nth_error_Some l i) as LEN.
+  rewrite H in LEN.
+  destruct (list.nth_lookup_or_length l i a).
+  - rewrite (List.nth_error_nth l i a H) in e.
+    assumption.
+  - intuition.
+* apply list.lookup_ge_None.
+  apply List.nth_error_None.
+  assumption.
+Qed.
+
+Lemma nth_error_rev A (l : list A) i x :
+  List.nth_error l i = Some x <-> List.nth_error (List.rev l) (List.length l - i - 1) = Some x /\ i < List.length l.
+destruct (lt_dec i (List.length l)) as [H|H].
+* rewrite List.nth_error_nth' with (d := x); auto.
+  rewrite List.nth_error_nth' with (d := x). 2: {
+    rewrite List.rev_length.
+    Lia.lia.
+  }
+  rewrite List.rev_nth. 2: Lia.lia.
+  replace (List.length l - S (List.length l - i - 1)) with i by Lia.lia.
+  tauto.
+* apply not_lt in H.
+  specialize (List.nth_error_None l i) as H'.
+  intuition; solve [congruence | Lia.lia].
+Qed.
+
+Lemma word_to_bools_get_bit : forall [n] (w : word n) (i : nat) x,
+  List.nth_error (word_to_bools w) i = Some x <-> get_bit w (n - i - 1) = x /\ i < n.
+intros.
+unfold word_to_bools, get_bit.
+specialize (bitvector.bv_to_bits_lookup_Some w (n - i - 1) x).
+rewrite nth_error_lookup.
+intro H.
+rewrite nth_error_rev.
+rewrite List.rev_involutive, List.rev_length.
+rewrite bitvector.bv_to_bits_length.
+rewrite Nnat.Nat2N.id.
+intuition.
+Qed.
+
+Lemma word_to_bools_nth_Some : forall [n] (w : word n) (i : nat) x, n > 0 ->
+  List.nth_error (word_to_bools w) i = Some x <-> x = N.testbit (word_to_N w) (N.of_nat (n - i - 1)) /\ i < n.
+intros.
+rewrite word_to_bools_get_bit.
+unfold get_bit, word_to_N.
+rewrite <- (Z2N.id (bitvector.bv_unsigned w)) at 1.
+rewrite <- nat_N_Z.
+rewrite Z.testbit_of_N.
+intuition.
+firstorder using bitvector.bv_unsigned_in_range.
+Qed.
+
+Lemma N_of_digits_limit l :
+  (Ascii.N_of_digits l < 2 ^ N.of_nat (List.length l))%N.
+induction l.
+* simpl. Lia.lia.
+* simpl (List.length _).
+  rewrite Nnat.Nat2N.inj_succ.
+  rewrite N.pow_succ_r'.
+  simpl (Ascii.N_of_digits _).
+  destruct (Ascii.N_of_digits l); destruct a; Lia.lia.
+Qed.
+
+Local Lemma nth_error_N_of_digits l i b :
+  List.nth_error l i = Some b <-> N.testbit (Ascii.N_of_digits l) (N.of_nat i) = b /\ i < List.length l.
+revert i.
+induction l.
+* destruct i; simpl; intuition.
+* destruct i.
+  - destruct a; simpl; destruct (Ascii.N_of_digits l); simpl; intuition.
+  - rewrite Nnat.Nat2N.inj_succ.
+    replace (Ascii.N_of_digits (a::l)) with (2 * Ascii.N_of_digits l + N.b2n a)%N. 2: {
+      simpl Ascii.N_of_digits at 2.
+      destruct (Ascii.N_of_digits l).
+      + destruct a; simpl; Lia.lia.
+      + destruct a; simpl; Lia.lia.
+    }
+    rewrite N.testbit_succ_r.
+    specialize (IHl i).
+    intuition.
+    simpl; Lia.lia.
+Qed.
+
+Lemma bools_to_word_get_bit : forall l i b,
+  List.nth_error l i = Some b <-> get_bit (bools_to_word l) (List.length l - i - 1) = b /\ i < List.length l.
+intros.
+unfold bools_to_word, get_bit, N_to_word.
+rewrite bitvector.Z_to_bv_unsigned.
+rewrite bitvector.bv_wrap_small. 2: {
+  split; [Lia.lia|].
+  unfold bitvector.bv_modulus.
+  specialize (N_of_digits_limit (List.rev l)).
+  rewrite List.rev_length.
+  Lia.lia.
+}
+erewrite <- nat_N_Z.
+rewrite Z.testbit_of_N.
+rewrite nth_error_rev.
+specialize (nth_error_N_of_digits (List.rev l) (List.length l - i - 1) b).
+rewrite List.rev_length.
+intuition.
+Qed.
+
+Lemma bools_to_word_nth_Some : forall (l : list bool) i b,
+  List.nth_error l i = Some b <-> b = N.testbit (word_to_N (bools_to_word l)) (N.of_nat (List.length l - i - 1)) /\ i < List.length l.
+intros.
+rewrite bools_to_word_get_bit.
+unfold get_bit, word_to_N.
+rewrite <- (Z2N.id (bitvector.bv_unsigned (bools_to_word l))) at 1. 2: {
+  specialize (bitvector.bv_unsigned_in_range _ (bools_to_word l)).
+  intuition.
+}
+rewrite <- nat_N_Z.
+rewrite Z.testbit_of_N.
+intuition.
+Qed.
 
 Definition slice {m} n (w : word m) i : word n := bitvector.bv_extract (N.of_nat i) _ w.
 Definition update_slice {m n} (w : word m) i (v : word n) : word m :=
