lib/coq/MachineWordInterface.v
@@ -8,6 +8,9 @@ Parameter ones : forall n, word n.
 Parameter get_bit : forall [n], word n -> nat -> bool.
 Parameter set_bit : forall [n], word n -> nat -> bool -> word n.
 
+Axiom get_bit_eq : forall [n] (w v : word n),
+  (forall i, i < n -> get_bit w i = get_bit v i) -> w = v.
+
 (* These are big-endian, in keeping with the Lem backend. *)
 Parameter word_to_bools : forall [n], word n -> list bool.
 Parameter bools_to_word : forall l : list bool, word (List.length l).
@@ -19,6 +22,19 @@ Parameter N_to_word : forall n, N -> word n.
 
 Axiom word_to_N_range : forall [n] (w : word n), (word_to_N w < 2 ^ N.of_nat n)%N.
 Axiom word_to_Z_range : forall [n] (w : word (S n)), (- 2 ^ Z.of_nat n <= word_to_Z w < 2 ^ Z.of_nat n)%Z.
+Axiom testbit_word_to_N_high : forall [n] (w: word n) i, (i >= N.of_nat n)%N ->
+  N.testbit (word_to_N w) i = false.
+
+Axiom word_to_bools_length : forall [n] (w : word n), List.length (word_to_bools w) = n.
+Axiom word_to_bools_get_bit : forall [n] (w : word n) (i : nat) x,
+  List.nth_error (word_to_bools w) i = Some x <-> get_bit w (n - i - 1) = x /\ i < n.
+Axiom word_to_bools_nth_Some : forall [n] (w : word n) (i : nat) x, n > 0 ->
+  List.nth_error (word_to_bools w) i = Some x <-> x = N.testbit (word_to_N w) (N.of_nat (n - i - 1)) /\ i < n.
+Axiom bools_to_word_get_bit : forall l i b,
+  List.nth_error l i = Some b <-> get_bit (bools_to_word l) (length l - i - 1) = b /\ i < length l.
+Axiom bools_to_word_nth_Some : forall (l : list bool) i b,
+  List.nth_error l i = Some b <-> b = N.testbit (word_to_N (bools_to_word l)) (N.of_nat (length l - i - 1)) /\ i < length l.
+
 
 Parameter slice : forall [m] n, word m -> nat -> word n.
 Parameter update_slice : forall [m] [n], word m -> nat -> word n -> word m.
